be more explicit in a flaky proof

ulib/FStar.UInt.fst
@@ -149,10 +149,15 @@ val mul_mod: #n:nat -> a:uint_t n -> b:uint_t n -> Tot (uint_t n)
 let mul_mod #n a b =
   (a * b) % (pow2 n)
 
+let lt_square_div_lt (a:nat) (b:pos) : Lemma
+  (requires (a < b * b))
+  (ensures (a / b < b))
+  = ()
+
 val mul_div: #n:nat -> a:uint_t n -> b:uint_t n -> Tot (uint_t n)
-#reset-options "--max_fuel 0 --max_ifuel 0 --z3rlimit 40"
 let mul_div #n a b =
   FStar.Math.Lemmas.lemma_mult_lt_sqr a b (pow2 n);
+  lt_square_div_lt (a * b) (pow2 n);
   (a * b) / (pow2 n)
 
 #reset-options "--max_fuel 0 --max_ifuel 0"
